TraceInclusions.v
@@ -1,0 +1,343 @@
+Require Import Kami.Syntax.
+Import ListNotations.
+Require Import Kami.Properties.
+Require Import Kami.PProperties.
+Require Import Kami.PPlusProperties.
+(*
+Properties.v:  Theorem simulationZeroAction:
+*)
+Theorem _StepSimulation (imp spec : Mod) (simRel : RegsT -> RegsT -> Prop)
+        (initRel : forall rimp : list RegT,
+            Forall2 regInit rimp (getAllRegisters imp)
+            -> exists rspec, Forall2 regInit rspec (getAllRegisters spec)
+                             /\ simRel rimp rspec) 
+        (NoDupRegs : NoDup (map fst (getAllRegisters imp)))
+        (stepSimulationNonZero : forall oImp lImp oImp',
+            Step imp oImp lImp ->
+            lImp <> nil ->
+            UpdRegs (map fst lImp) oImp oImp' ->
+            forall oSpec,
+              simRel oImp oSpec ->
+              exists lSpec oSpec',
+                Step spec oSpec lSpec /\
+                UpdRegs (map fst lSpec) oSpec oSpec' /\
+                simRel oImp' oSpec' /\ WeakInclusion lImp lSpec) :
+  TraceInclusion imp spec.
+Proof.
+  eauto using StepSimulation.
+Qed.
+
+Theorem _simulationZero (imp spec : BaseModule) (simRel : RegsT -> RegsT -> Prop)
+        (initRel : forall rimp : list RegT,
+            Forall2 regInit rimp (getAllRegisters imp)
+            -> exists rspec, Forall2 regInit rspec (getAllRegisters spec)
+                             /\ simRel rimp rspec) 
+        (NoDupRegs : NoDup (map fst (getAllRegisters imp)))
+        (NoMeths : getMethods imp = [])
+        (NoMethsSpec: getMethods spec = [])
+        (simulation : forall oImp uImp rleImp csImp oImp',
+            Substeps imp oImp [(uImp, (Rle rleImp, csImp))] ->
+            UpdRegs [uImp] oImp oImp' ->
+            forall oSpec,
+              simRel oImp oSpec ->
+              (getKindAttr oSpec = getKindAttr (getRegisters spec) /\ simRel oImp' oSpec
+               /\ csImp = [])
+              \/ exists uSpec rleSpec oSpec',
+                  Substeps spec oSpec [(uSpec, (Rle rleSpec, csImp))] /\
+                  UpdRegs [uSpec] oSpec oSpec' /\
+                  simRel oImp' oSpec') :
+  TraceInclusion (Base imp) (Base spec).
+Proof.
+  eauto using simulationZero.
+Qed.
+
+Theorem _flatten_WfMod m :
+  WfMod m -> WfMod (flatten m).
+Proof.
+  eauto using flatten_WfMod.
+Qed.
+
+Theorem _TraceInclusion_flatten_r (m : ModWf) :
+  TraceInclusion m (flattened_ModWf m).
+Proof.
+  eauto using TraceInclusion_flatten_r.
+Qed.
+
+Theorem _TraceInclusion_flatten_l (m : ModWf) :
+  TraceInclusion (flattened_ModWf m) m.
+Proof.
+  eauto using TraceInclusion_flatten_l.
+Qed.
+
+Theorem _ModularSubstitution (a b a' b' : Mod)
+        (SameList_a : forall x,
+            (In x (map fst (getAllMethods a)) /\
+             ~ In x (getHidden a)) <->
+            (In x (map fst (getAllMethods a')) /\
+             ~ In x (getHidden a')))
+        (SameList_b : forall x,
+            (In x (map fst (getAllMethods b)) /\
+             ~ In x (getHidden b)) <->
+            (In x (map fst (getAllMethods b')) /\
+             ~ In x (getHidden b')))
+        (wfAConcatB : WfMod (ConcatMod a b))
+        (wfA'ConcatB' : WfMod (ConcatMod a' b')):
+  TraceInclusion a a' ->
+  TraceInclusion b b' ->
+  TraceInclusion (ConcatMod a b) (ConcatMod a' b').
+Proof.
+  eauto using ModularSubstitution.
+Qed.
+
+Theorem _simulationZeroAct (imp spec : BaseModuleWf) (simRel : RegsT -> RegsT -> Prop)
+        (simRelGood : forall oImp oSpec : RegsT,
+        simRel oImp oSpec -> getKindAttr oSpec = getKindAttr (getRegisters spec))
+        (initRel : forall rimp : list RegT,
+            Forall2 regInit rimp (getAllRegisters imp)
+            -> exists rspec, Forall2 regInit rspec (getAllRegisters spec)
+                             /\ simRel rimp rspec) 
+        (NoMeths : getMethods imp = [])
+        (NoMethsSpec: getMethods spec = [])
+        (simulation : forall oImp rImp uImp rleImp csImp oImp' aImp,
+            In (rleImp, aImp) (getRules imp) ->
+            SemAction oImp (aImp type) rImp uImp csImp WO ->
+            UpdRegs [uImp] oImp oImp' ->
+            forall oSpec,
+              simRel oImp oSpec ->
+              (simRel oImp' oSpec /\ csImp = [])
+              \/ (exists rleSpec aSpec,
+                  In (rleSpec, aSpec) (getRules spec) /\
+                  exists rSpec uSpec,
+                    SemAction oSpec (aSpec type) rSpec uSpec csImp WO /\
+                    exists oSpec',
+                      UpdRegs [uSpec] oSpec oSpec' /\
+                      simRel oImp' oSpec')):
+  TraceInclusion (Base imp) (Base spec).
+Proof.
+  eauto using simulationZeroAct.
+Qed.
+
+Theorem _simulationGen (imp spec : BaseModuleWf) (NoSelfCalls : NoSelfCallBaseModule spec)
+        (simRel : RegsT -> RegsT -> Prop)
+        (simRelGood : forall oImp oSpec : RegsT,
+            simRel oImp oSpec -> getKindAttr oSpec = getKindAttr (getRegisters spec))
+        (initRel : forall rimp : list RegT,
+            Forall2 regInit rimp (getAllRegisters imp)
+            -> exists rspec, Forall2 regInit rspec (getAllRegisters spec)
+                             /\ simRel rimp rspec)
+        (simulationRule :
+           forall oImp rImp uImp rleImp csImp oImp' aImp,
+             In (rleImp, aImp) (getRules imp) ->
+             SemAction oImp (aImp type) rImp uImp csImp WO ->
+             UpdRegs [uImp] oImp oImp' ->
+             forall oSpec,
+               simRel oImp oSpec ->
+               ((simRel oImp' oSpec /\ csImp = []) \/
+                (exists rleSpec aSpec,
+                    In (rleSpec, aSpec) (getRules spec) /\
+                    exists rSpec uSpec,
+                      SemAction oSpec (aSpec type) rSpec uSpec csImp WO /\
+                      exists oSpec',
+                        UpdRegs [uSpec] oSpec oSpec' /\
+                        simRel oImp' oSpec')))
+        (simulationMeth :
+           forall oImp rImp uImp meth csImp oImp' sign aImp arg ret,
+             In (meth, existT _ sign aImp) (getMethods imp) ->
+             SemAction oImp (aImp type arg) rImp uImp csImp ret ->
+             UpdRegs [uImp] oImp oImp' ->
+             forall oSpec,
+               simRel oImp oSpec ->
+               exists aSpec rSpec uSpec,
+                 In (meth, existT _ sign aSpec) (getMethods spec) /\
+                 SemAction oSpec (aSpec type arg) rSpec uSpec csImp ret /\
+                 exists oSpec',
+                   UpdRegs [uSpec] oSpec oSpec' /\
+                   simRel oImp' oSpec')
+        (notMethMeth :
+           forall oImp rImpl1 uImpl1 meth1 sign1 aImp1 arg1 ret1 csImp1
+                  rImpl2 uImpl2 meth2 sign2 aImp2 arg2 ret2 csImp2,
+             In (meth1, existT _ sign1 aImp1) (getMethods imp) ->
+             SemAction oImp (aImp1 type arg1) rImpl1 uImpl1 csImp1 ret1 ->
+             In (meth2, existT _ sign2 aImp2) (getMethods imp) ->
+             SemAction oImp (aImp2 type arg2) rImpl2 uImpl2 csImp2 ret2 ->
+             exists k, In k (map fst uImpl1) /\ In k (map fst uImpl2))
+        (notRuleMeth :
+           forall oImp rImpl1 uImpl1 rleImpl1 aImp1 csImp1
+                  rImpl2 uImpl2 meth2 sign2 aImp2 arg2 ret2 csImp2,
+             In (rleImpl1, aImp1) (getRules imp) ->
+             SemAction oImp (aImp1 type) rImpl1 uImpl1 csImp1 WO ->
+             In (meth2, existT _ sign2 aImp2) (getMethods imp) ->
+             SemAction oImp (aImp2 type arg2) rImpl2 uImpl2 csImp2 ret2 ->
+             exists k, In k (map fst uImpl1) /\ In k (map fst uImpl2)) :
+  TraceInclusion (Base imp) (Base spec).
+Proof.
+  eauto using simulationGen.
+Qed.
+
+Theorem _simulationGeneralEx (imp spec: BaseModuleWf) (NoSelfCalls: NoSelfCallBaseModule spec)
+        (simRel: RegsT -> RegsT -> Prop)
+        (simRelGood: forall oImp oSpec,
+            simRel oImp oSpec -> getKindAttr oSpec = getKindAttr (getRegisters spec))
+        (simRelImpGood: forall oImp oSpec,
+            simRel oImp oSpec -> getKindAttr oImp = getKindAttr (getRegisters imp))
+        (initRel: forall rimp,
+            Forall2 regInit rimp (getRegisters imp) ->
+            exists rspec, Forall2 regInit rspec (getRegisters spec) /\ simRel rimp rspec)
+        (simulationRule:
+           forall oImp rImp uImp rleImp csImp aImp,
+             In (rleImp, aImp) (getRules imp) ->
+             SemAction oImp (aImp type) rImp uImp csImp WO ->
+             forall oSpec,
+               simRel oImp oSpec ->
+               ((simRel (doUpdRegs uImp oImp) oSpec /\ csImp = []) \/
+                (exists rleSpec aSpec,
+                    In (rleSpec, aSpec) (getRules spec) /\
+                    exists rSpec uSpec,
+                      SemAction oSpec (aSpec type) rSpec uSpec csImp WO /\
+                      exists oSpec',
+                        UpdRegs [uSpec] oSpec oSpec' /\
+                        simRel (doUpdRegs uImp oImp) oSpec')))
+        (simulationMeth:
+           forall oImp rImp uImp meth csImp sign aImp arg ret,
+             In (meth, existT _ sign aImp) (getMethods imp) ->
+             SemAction oImp (aImp type arg) rImp uImp csImp ret ->
+             forall oSpec,
+               simRel oImp oSpec ->
+               exists aSpec rSpec uSpec,
+                 In (meth, existT _ sign aSpec) (getMethods spec) /\
+                 SemAction oSpec (aSpec type arg) rSpec uSpec csImp ret /\
+                 exists oSpec',
+                   UpdRegs [uSpec] oSpec oSpec' /\
+                   simRel (doUpdRegs uImp oImp) oSpec')
+        (notMethMeth:
+           forall oImp rImpl1 uImpl1 meth1 sign1 aImp1 arg1 ret1 csImp1
+                  rImpl2 uImpl2 meth2 sign2 aImp2 arg2 ret2 csImp2,
+             In (meth1, existT _ sign1 aImp1) (getMethods imp) ->
+             SemAction oImp (aImp1 type arg1) rImpl1 uImpl1 csImp1 ret1 ->
+             In (meth2, existT _ sign2 aImp2) (getMethods imp) ->
+             SemAction oImp (aImp2 type arg2) rImpl2 uImpl2 csImp2 ret2 ->
+             exists k, In k (map fst uImpl1) /\ In k (map fst uImpl2))
+        (notRuleMeth:
+           forall oImp rImpl1 uImpl1 rleImpl1 aImp1 csImp1
+                  rImpl2 uImpl2 meth2 sign2 aImp2 arg2 ret2 csImp2,
+             In (rleImpl1, aImp1) (getRules imp) ->
+             SemAction oImp (aImp1 type) rImpl1 uImpl1 csImp1 WO ->
+             In (meth2, existT _ sign2 aImp2) (getMethods imp) ->
+             SemAction oImp (aImp2 type arg2) rImpl2 uImpl2 csImp2 ret2 ->
+             exists k, In k (map fst uImpl1) /\ In k (map fst uImpl2)) :
+  TraceInclusion (Base imp) (Base spec).
+Proof.
+  eauto using simulationGeneralEx.
+Qed.
+
+Theorem _simulationZeroA (imp spec: BaseModuleWf) (simRel: RegsT -> RegsT -> Prop)
+        (simRelGood: forall oImp oSpec,
+            simRel oImp oSpec ->
+            getKindAttr oSpec = getKindAttr (getRegisters spec))
+        (simRelImpGood: forall oImp oSpec,
+            simRel oImp oSpec ->
+            getKindAttr oImp = getKindAttr (getRegisters imp))
+        (initRel: forall rimp,
+            Forall2 regInit rimp (getRegisters imp) ->
+            exists rspec, Forall2 regInit rspec (getRegisters spec) /\
+                          simRel rimp rspec)
+        (NoMeths: getMethods imp = [])
+        (NoMethsSpec: getMethods spec = [])
+        (simulation:
+           forall oImp rImp uImp rleImp csImp aImp,
+             In (rleImp, aImp) (getRules imp) ->
+             SemAction oImp (aImp type) rImp uImp csImp WO ->
+             forall oSpec,
+               simRel oImp oSpec ->
+               ((simRel (doUpdRegs uImp oImp) oSpec /\ csImp = []) \/
+                (exists rleSpec aSpec,
+                    In (rleSpec, aSpec) (getRules spec) /\
+                    exists rSpec uSpec,
+                      SemAction oSpec (aSpec type) rSpec uSpec csImp WO /\
+                      exists oSpec',
+                        UpdRegs [uSpec] oSpec oSpec' /\
+                        simRel (doUpdRegs uImp oImp) oSpec'))) :
+  TraceInclusion (Base imp) (Base spec).
+Proof.
+  eauto using simulationZeroA.
+Qed.
+
+Theorem _simulationGeneral (imp spec: BaseModuleWf) (NoSelfCalls: NoSelfCallBaseModule spec)
+        (simRel: RegsT -> RegsT -> Prop)
+        (simRelGood: forall oImp oSpec,
+            simRel oImp oSpec -> getKindAttr oSpec = getKindAttr (getRegisters spec))
+        (simRelImpGood: forall oImp oSpec,
+            simRel oImp oSpec -> getKindAttr oImp = getKindAttr (getRegisters imp))
+        (initRel: forall rimp,
+            Forall2 regInit rimp (getRegisters imp) ->
+            exists rspec, Forall2 regInit rspec (getRegisters spec) /\ simRel rimp rspec)
+        (simulationRule:
+           forall oImp rImp uImp rleImp csImp aImp,
+             In (rleImp, aImp) (getRules imp) ->
+             SemAction oImp (aImp type) rImp uImp csImp WO ->
+             forall oSpec,
+               simRel oImp oSpec ->
+               ((simRel (doUpdRegs uImp oImp) oSpec /\ csImp = []) \/
+                (exists rleSpec aSpec,
+                    In (rleSpec, aSpec) (getRules spec) /\
+                    exists rSpec uSpec,
+                      SemAction oSpec (aSpec type) rSpec uSpec csImp WO /\
+                      simRel (doUpdRegs uImp oImp) (doUpdRegs uSpec oSpec))))
+        (simulationMeth:
+           forall oImp rImp uImp meth csImp sign aImp arg ret,
+             In (meth, existT _ sign aImp) (getMethods imp) ->
+             SemAction oImp (aImp type arg) rImp uImp csImp ret ->
+             forall oSpec,
+               simRel oImp oSpec ->
+               exists aSpec rSpec uSpec,
+                 In (meth, existT _ sign aSpec) (getMethods spec) /\
+                 SemAction oSpec (aSpec type arg) rSpec uSpec csImp ret /\
+                 simRel (doUpdRegs uImp oImp) (doUpdRegs uSpec oSpec))
+        (notMethMeth:
+           forall oImp rImpl1 uImpl1 meth1 sign1 aImp1 arg1 ret1 csImp1
+                  rImpl2 uImpl2 meth2 sign2 aImp2 arg2 ret2 csImp2,
+             In (meth1, existT _ sign1 aImp1) (getMethods imp) ->
+             SemAction oImp (aImp1 type arg1) rImpl1 uImpl1 csImp1 ret1 ->
+             In (meth2, existT _ sign2 aImp2) (getMethods imp) ->
+             SemAction oImp (aImp2 type arg2) rImpl2 uImpl2 csImp2 ret2 ->
+             exists k, In k (map fst uImpl1) /\ In k (map fst uImpl2))
+        (notRuleMeth:
+           forall oImp rImpl1 uImpl1 rleImpl1 aImp1 csImp1
+                  rImpl2 uImpl2 meth2 sign2 aImp2 arg2 ret2 csImp2,
+             In (rleImpl1, aImp1) (getRules imp) ->
+             SemAction oImp (aImp1 type) rImpl1 uImpl1 csImp1 WO ->
+             In (meth2, existT _ sign2 aImp2) (getMethods imp) ->
+             SemAction oImp (aImp2 type arg2) rImpl2 uImpl2 csImp2 ret2 ->
+             exists k, In k (map fst uImpl1) /\ In k (map fst uImpl2)) :
+  TraceInclusion (Base imp) (Base spec).
+Proof.
+  eauto using simulationGeneral.
+Qed.
+
+Theorem _simulationZeroAction (imp spec: BaseModuleWf) (simRel: RegsT -> RegsT -> Prop)
+        (simRelGood: forall oImp oSpec,
+            simRel oImp oSpec -> getKindAttr oSpec = getKindAttr (getRegisters spec))
+        (simRelImpGood: forall oImp oSpec,
+            simRel oImp oSpec -> getKindAttr oImp = getKindAttr (getRegisters imp))
+        (initRel: forall rimp,
+            Forall2 regInit rimp (getRegisters imp) ->
+            exists rspec, Forall2 regInit rspec (getRegisters spec) /\
+                          simRel rimp rspec)
+        (NoMeths: getMethods imp = [])
+        (NoMethsSpec: getMethods spec = [])
+        (simulation:
+           forall oImp rImp uImp rleImp csImp aImp,
+             In (rleImp, aImp) (getRules imp) ->
+             SemAction oImp (aImp type) rImp uImp csImp WO ->
+             forall oSpec,
+               simRel oImp oSpec ->
+               ((simRel (doUpdRegs uImp oImp) oSpec /\ csImp = []) \/
+                (exists rleSpec aSpec,
+                    In (rleSpec, aSpec) (getRules spec) /\
+                    exists rSpec uSpec,
+                      SemAction oSpec (aSpec type) rSpec uSpec csImp WO /\
+                      simRel (doUpdRegs uImp oImp) (doUpdRegs uSpec oSpec)))) :
+  TraceInclusion (Base imp) (Base spec).
+Proof.
+  eauto using simulationZeroAction.
+Qed.
